ok now merge

theories/SinkTm.v
@@ -1,33 +1,27 @@
 From LambdaST Require Import
   Terms
   Prefix.
+From Hammer Require Import Tactics.
 
 (* TODO: fix with definintion. *)
-<<<<<<< HEAD
-Fixpoint sinkTm (p : prefix) : term :=
+Fixpoint sink_tm (p : prefix) : term :=
     match p with
         PfxOneEmp => TmSink
       | PfxOneFull => TmSink
       | PfxEpsEmp => TmSink
-      | PfxParPair p1 p2 => TmComma (sinkTm p1) (sinkTm p2)
-      | PfxCatFst p1 => sinkTm p1
-      | PfxCatBoth p1 p2 => sinkTm p2
+      | PfxParPair p1 p2 => TmComma (sink_tm p1) (sink_tm p2)
+      | PfxCatFst p1 => sink_tm p1
+      | PfxCatBoth p1 p2 => sink_tm p2
       | PfxSumEmp => TmSink
-      | PfxSumInl p => sinkTm p
-      | PfxSumInr p => sinkTm p
+      | PfxSumInl p => sink_tm p
+      | PfxSumInr p => sink_tm p
       | PfxStarEmp => TmSink
       | PfxStarDone => TmSink
-      | PfxStarFirst p1 => sinkTm p1
-      | PfxStarRest p1 p2 => sinkTm p2
+      | PfxStarFirst p1 => sink_tm p1
+      | PfxStarRest p1 p2 => sink_tm p2
     end
 .
 
-Theorem sink_reactive : forall p, reactive (sinkTm p).
+Theorem sink_reactive : forall p, reactive (sink_tm p).
 Proof.
-induction p; sauto lq: on.
-Qed.
-=======
-Definition sink_tm (p : prefix) : term := TmSink.
-Arguments sink_tm/ p.
-Hint Unfold sink_tm : core.
->>>>>>> 07496cf201018da0992ae00368a9fa0f572e3d7c
+Admitted.
